Upstream lemmas about [list] w/ [N] from UMX

theories/prelude/list_numbers.v
@@ -1,3 +1,4 @@
+From stdpp Require Import propset option.
 From bedrock.prelude Require Import base.
 From bedrock.prelude Require Export list numbers.
 
@@ -19,6 +20,8 @@ Definition lengthN {A} xs := N.of_nat (length (A := A) xs).
 Definition resizeN {A} n := resize (A := A) (N.to_nat n).
 Definition rotateN {A} n xs :=
   dropN (A := A) (n mod lengthN xs) xs ++ takeN (A := A) (n mod lengthN xs) xs.
+#[global] Instance lookupN {A}: Lookup N A (list A) := fun i xs => lookup (N.to_nat i) xs.
+
 
 Lemma fmap_lengthN {A B} (f : A → B) (l : list A) :
   lengthN (f <$> l) = lengthN l.
@@ -86,7 +89,7 @@ Proof. by intros [-> _]%elem_of_replicate. Qed.
 Section listN.
   Context {A : Type}.
 
-  Implicit Type (x : A) (n m : N).
+  Implicit Type (x : A) (xs : list A) (i n m k : N).
 
   Lemma N2Nat_inj_le n m :
     n ≤ m ->
@@ -100,7 +103,7 @@ Section listN.
     rewrite elem_of_seq. lia.
   Qed.
 
-  Lemma Forall_seqN P (i n : N) :
+  Lemma Forall_seqN P i n :
     List.Forall P (seqN i n) ↔ (∀ j : N, i <= j < i + n → P j).
   Proof. rewrite Forall_forall. by setoid_rewrite elem_of_seqN. Qed.
 
@@ -112,6 +115,33 @@ Section listN.
   Lemma cons_lengthN x xs :
     lengthN (x :: xs) = N.succ (lengthN xs).
   Proof. by rewrite /lengthN cons_length Nat2N.inj_succ. Qed.
+
+  Lemma replicateN_zero x :
+    replicateN 0 x = [].
+  Proof. reflexivity. Qed.
+
+  Lemma replicateN_succ n x :
+    replicateN (n + 1) x = x :: replicateN n x.
+  Proof. by rewrite /replicateN N.add_1_r N2Nat.inj_succ/=. Qed.
+
+  Lemma replicateN_succ' n x :
+    replicateN (n + 1) x = replicateN n x ++ [x].
+  Proof.
+    elim/N.induction: n=> [|n IH]//.
+    rewrite -N.add_1_r replicateN_succ {2}replicateN_succ/=.
+    by rewrite IH.
+  Qed.
+
+  Definition replicateN_simpl :=
+    (@replicateN_zero, @replicateN_succ).
+
+  Lemma replicateN_cons n x :
+    0 < n ->
+    replicateN n x = x :: replicateN (n - 1) x.
+  Proof.
+    rewrite /replicateN N2Nat.inj_sub. elim/N.case_analysis: n=> [|n']// _.
+    by rewrite N2Nat.inj_succ/= Nat.sub_0_r.
+  Qed.
 
   (* Lift all theory about [drop] and [replicate] interaction. *)
   Lemma dropN_replicateN n m x :
@@ -131,13 +161,63 @@ Section listN.
     takeN n (replicateN (n + m) x) = replicateN n x.
   Proof. by rewrite /takeN /replicateN N2Nat.inj_add take_replicate_plus. Qed.
 
+  Lemma to_nat_lengthN xs :
+    N.to_nat (lengthN xs) = length xs.
+  Proof. by rewrite /lengthN Nat2N.id. Qed.
+
+  Lemma lengthN_fold xs :
+    N.of_nat (length xs) = lengthN xs.
+  Proof. reflexivity. Qed.
+
+  Lemma lengthN_nil :
+    lengthN (A := A) [] = 0.
+  Proof. reflexivity. Qed.
+
+  Lemma lengthN_cons x xs :
+    lengthN (x :: xs) = (lengthN xs) + 1.
+  Proof. rewrite N.add_1_r /lengthN/=. by case: (length xs). Qed.
+
+  Lemma lengthN_one x :
+    lengthN [x] = 1.
+  Proof. reflexivity. Qed.
+
+  Lemma lengthN_app xs1 xs2 :
+    lengthN (xs1 ++ xs2) = lengthN xs1 + lengthN xs2.
+  Proof. by rewrite /lengthN app_length Nat2N.inj_add. Qed.
+
+  Lemma lengthN_map {B} (f : A -> B) xs :
+    lengthN (map f xs) = lengthN xs.
+  Proof. by rewrite /lengthN map_length. Qed.
+
+  Lemma lengthN_dropN k xs :
+    lengthN (dropN k xs) = lengthN xs - k.
+  Proof. by rewrite /lengthN/dropN drop_length Nat2N.inj_sub N2Nat.id. Qed.
+
+  Lemma lengthN_takeN k xs :
+    lengthN (takeN k xs) = k `min` lengthN xs.
+  Proof. by rewrite /lengthN/takeN take_length Nat2N.inj_min N2Nat.id. Qed.
+
+  Lemma lengthN_rotateN k xs :
+    lengthN (rotateN k xs) = lengthN xs.
+  Proof. rewrite /rotateN lengthN_app lengthN_dropN lengthN_takeN. lia. Qed.
+
+  Lemma lengthN_replicateN n x :
+    lengthN (replicateN n x) = n.
+  Proof. by rewrite /lengthN/replicateN replicate_length N2Nat.id. Qed.
+
+  Definition lengthN_simpl :=
+    (@lengthN_fold,
+     @lengthN_nil, @lengthN_cons,
+     @lengthN_app, @lengthN_map,
+     @lengthN_dropN, @lengthN_takeN,
+     @lengthN_rotateN, @lengthN_replicateN).
+
   Lemma resizeN_spec l n x :
     resizeN n x l = takeN n l ++ replicateN (n - lengthN l) x.
   Proof.
     by rewrite /resizeN /replicateN resize_spec !N2Nat.inj_sub Nat2N.id.
   Qed.
 
-  (* Part of the theory of [resize], it's rather large. *)
   Lemma resizeN_all l x : resizeN (lengthN l) x l = l.
   Proof. by rewrite /resizeN /lengthN Nat2N.id resize_all. Qed.
 
@@ -159,7 +239,60 @@ Section listN.
     resizeN n x (resizeN n x l) = resizeN n x l.
   Proof. apply resize_idemp. Qed.
 
-  (* Lift all theory about [drop] and [resize] interaction. *)
+  Lemma resizeN_plusN l n m x :
+    resizeN (n + m) x l = resizeN n x l ++ resizeN m x (dropN n l).
+  Proof. by rewrite /resizeN /dropN N2Nat.inj_add resize_plus. Qed.
+
+  Lemma resizeN_takeN_eq l n x :
+    resizeN n x (takeN n l) = resizeN n x l.
+  Proof. apply resize_take_eq. Qed.
+
+  Lemma resizeN_le l n x :
+    n <= lengthN l ->
+    resizeN n x l = takeN n l.
+  Proof. move=> /N2Nat_inj_le. rewrite to_nat_lengthN. apply resize_le. Qed.
+
+  Lemma resizeN_takeN_le l n m x :
+    (n <= m) → resizeN n x (takeN m l) = resizeN n x l.
+  Proof. move=> /N2Nat_inj_le. apply resize_take_le. Qed.
+
+  Lemma dropN_lengthN n xs :
+    lengthN xs <= n -> dropN n xs = [].
+  Proof.
+    rewrite /lengthN/dropN=> /N2Nat_inj_le. rewrite Nat2N.id.
+    by apply: drop_ge.
+  Qed.
+
+  Lemma dropN_zero xs :
+    dropN 0 xs = xs.
+  Proof. reflexivity. Qed.
+
+  Lemma dropN_one x xs :
+    dropN 1 (x :: xs) = xs.
+  Proof. reflexivity. Qed.
+
+  Lemma dropN_nil n :
+    dropN (A := A) n [] = [].
+  Proof. rewrite /dropN. by case: (N.to_nat _). Qed.
+
+  Lemma dropN_app n xs1 xs2 :
+    dropN n (xs1 ++ xs2) = dropN n xs1 ++ dropN (n - lengthN xs1) xs2.
+  Proof.
+    rewrite /dropN/lengthN N2Nat.inj_sub Nat2N.id. by apply: skipn_app.
+  Qed.
+
+  Lemma dropN_dropN n m xs :
+    dropN n (dropN m xs) = dropN (n + m) xs.
+  Proof.
+    rewrite /dropN N2Nat.inj_add Nat.add_comm. by apply: drop_drop.
+  Qed.
+
+  Lemma dropN_takeN n m xs :
+    dropN n (takeN m xs) = takeN (m - n) (dropN n xs).
+  Proof.
+    rewrite /dropN/takeN N2Nat.inj_sub. by apply: skipn_firstn_comm.
+  Qed.
+
   Lemma dropN_resizeN_plus l m n x :
     dropN n (resizeN (n + m) x l) = resizeN m x (dropN n l).
   Proof. by rewrite /dropN /resizeN N2Nat.inj_add drop_resize_plus. Qed.
@@ -172,18 +305,46 @@ Section listN.
     by rewrite /dropN /resizeN drop_resize_le // N2Nat.inj_sub.
   Qed.
 
-  Lemma resizeN_plusN l n m x :
-    resizeN (n + m) x l = resizeN n x l ++ resizeN m x (dropN n l).
-  Proof. by rewrite /resizeN /dropN N2Nat.inj_add resize_plus. Qed.
+  Lemma takeN_zero xs :
+    takeN 0 xs = [].
+  Proof. reflexivity. Qed.
 
-  (* Lift all theory about [take] and [resize] interaction. *)
+  Lemma takeN_one x xs :
+    takeN 1 (x :: xs) = [x].
+  Proof. reflexivity. Qed.
+
+  Lemma takeN_nil n :
+    takeN (A := A) n [] = [].
+  Proof. rewrite /takeN. by case: (N.to_nat _). Qed.
+
+  Lemma takeN_lengthN n xs :
+    lengthN xs <= n -> takeN n xs = xs.
+  Proof.
+    rewrite /lengthN/takeN=> /N2Nat_inj_le. rewrite Nat2N.id.
+    by apply: take_ge.
+  Qed.
+
+  Lemma takeN_app n xs1 xs2 :
+    takeN n (xs1 ++ xs2) = takeN n xs1 ++ takeN (n - lengthN xs1) xs2.
+  Proof.
+    rewrite /takeN/lengthN N2Nat.inj_sub Nat2N.id. by apply: firstn_app.
+  Qed.
+
+  Lemma takeN_takeN n m xs :
+    takeN n (takeN m xs) = takeN (n `min` m) xs.
+  Proof.
+    rewrite /takeN N2Nat.inj_min. by apply: take_take.
+  Qed.
+
+  Lemma takeN_dropN n m xs :
+    takeN n (dropN m xs) = dropN m (takeN (m + n) xs).
+  Proof.
+    rewrite /dropN/takeN N2Nat.inj_add. by apply: firstn_skipn_comm.
+  Qed.
+
   Lemma takeN_resizeN_eq l n x :
     takeN n (resizeN n x l) = resizeN n x l.
   Proof. apply take_resize_eq. Qed.
-
-  Lemma resizeN_takeN_eq l n x :
-    resizeN n x (takeN n l) = resizeN n x l.
-  Proof. apply resize_take_eq. Qed.
 
   Lemma takeN_resizeN l n m x :
     takeN n (resizeN m x l) = resizeN (n `min` m) x l.
@@ -193,25 +354,270 @@ Section listN.
     takeN n (resizeN (n + m) x l) = resizeN n x l.
   Proof. by rewrite /takeN /resizeN N2Nat.inj_add take_resize_plus. Qed.
 
-  Lemma to_nat_lengthN (l : list A) :
-    N.to_nat (lengthN l) = length l.
-  Proof. by rewrite /lengthN Nat2N.id. Qed.
-
-  Lemma resizeN_le l n x :
-    n <= lengthN l ->
-    resizeN n x l = takeN n l.
-  Proof. move=> /N2Nat_inj_le. rewrite to_nat_lengthN. apply resize_le. Qed.
-
   Lemma takeN_resizeN_le l n m x  :
     n ≤ m →
     takeN n (resizeN m x l) = resizeN n x l.
   Proof. move=> /N2Nat_inj_le. apply take_resize_le. Qed.
 
-  Lemma resizeN_takeN_le l n m x :
-    (n <= m) → resizeN n x (takeN m l) = resizeN n x l.
-  Proof. move=> /N2Nat_inj_le. apply resize_take_le. Qed.
+  Lemma rotateN_fold k xs :
+    rotate (N.to_nat k) xs = rotateN k xs.
+  Proof.
+    rewrite /rotateN/rotate/dropN/takeN.
+    case: xs=> [|x xs]; first by rewrite !drop_nil !take_nil.
+    rewrite -Z_N_nat Z2N.inj_mod//; last by lia.
+    by rewrite N_nat_Z N2Z.id -Z_nat_N Nat2Z.id lengthN_fold.
+  Qed.
 
-  (* resizeN_spec is above *)
+  Definition head_list {A} (xs : list A) := option_list (hd_error xs).
+
+  Lemma tail_drop xs : tail xs = drop 1 xs.
+  Proof. reflexivity. Qed.
+
+  Lemma head_take xs : head_list xs = take 1 xs.
+  Proof. by case: xs. Qed.
+
+  Lemma rotateN_iter k xs :
+    rotateN k xs = N.iter k (fun xs => tail xs ++ head_list xs) xs.
+  Proof.
+    elim/N.induction: k xs=> [|k IH] xs.
+    { by rewrite /rotateN/rotate/= app_nil_r. }
+    rewrite N.iter_succ//= -IH -N.add_1_r.
+    rewrite -!rotateN_fold /rotate tail_drop head_take.
+    case: xs=> [|x1 xs]; first by do !rewrite drop_nil take_nil.
+    case: xs=> [|x2 xs]; first by rewrite !Z.mod_1_r/=.
+    set n := length (x1 :: x2 :: xs). rewrite !N_nat_Z.
+    have ?: (0%nat < n)%Z by apply: inj_lt; apply: Nat.lt_0_succ.
+    have ?: (1 < n)%Z by rewrite /n/=; lia.
+    have ?: (0 <= k)%Z by apply: N2Z.is_nonneg.
+    have ?: (0 <= k `mod` n < n)%Z by apply: Z.mod_pos_bound.
+    have ?: (1 <= n - Z.to_nat (k `mod` n))%nat by lia.
+    rewrite drop_app_le; last by rewrite drop_length -/n.
+    rewrite take_app_le; last by rewrite drop_length -/n.
+    rewrite drop_drop -app_assoc take_take_drop.
+    rewrite N2Z.inj_add/= -Zplus_mod_idemp_l.
+    case/decide: (k `mod` n + 1 = n)%Z=> E.
+    - rewrite E Z_mod_same_full/=.
+      rewrite -[1%nat]/(Z.to_nat 1) -Z2Nat.inj_add//; last by lia.
+      rewrite E Nat2Z.id drop_all firstn_all.
+      by rewrite app_nil_l app_nil_r.
+    - rewrite Z.mod_small; last by lia.
+      by rewrite -[1%nat]/(Z.to_nat 1) -Z2Nat.inj_add//; last by lia.
+  Qed.
+
+  Lemma rotateN_nil k :
+      rotateN (A := A) k [] = [].
+  Proof. by rewrite /rotateN/rotate/= dropN_nil takeN_nil. Qed.
+
+  Lemma rotateN_singleton k x :
+    rotateN k [x] = [x].
+  Proof. by rewrite -rotateN_fold /rotate Z.mod_1_r/=. Qed.
+
+  Lemma rotateN_zero xs :
+    rotateN 0 xs = xs.
+  Proof.
+    case: xs=> [|x xs]; first by rewrite rotateN_nil.
+    by rewrite -rotateN_fold /rotate Z.mod_0_l//= app_nil_r.
+  Qed.
+
+  Lemma rotateN_one x xs :
+    rotateN 1 (x :: xs) = xs ++ [x].
+  Proof.
+    rewrite -rotateN_fold /rotate [length (x :: xs)]/=.
+    set n := S _. case/Z.lt_eq_cases: (ltac:(lia) : (1 <= n)%Z)=> H.
+    - by rewrite Z.mod_1_l//.
+    - rewrite -H/= app_nil_r. subst n. case: xs H=> [|??]//=. lia.
+  Qed.
+
+  Lemma rotateN_lengthN k xs :
+    k = lengthN xs ->
+    rotateN k xs = xs.
+  Proof.
+    move=> -> {k}. rewrite -rotateN_fold /rotate /lengthN Nat2N.id.
+    rewrite Z_mod_same_full Z2Nat.inj_0/=. by apply: app_nil_r.
+  Qed.
+
+  Lemma rotateN_modulo k xs :
+    rotateN (k `mod` lengthN xs) xs = rotateN k xs.
+  Proof.
+    case: xs=> [|x xs]; first by rewrite !rotateN_nil.
+    set xs' := x :: xs. rewrite -!rotateN_fold /rotate/lengthN.
+    by rewrite !N_nat_Z N2Z.inj_mod// nat_N_Z Zmod_mod.
+  Qed.
+
+  Lemma rotateN_modulo' k xs :
+    rotateN (Z.to_N (k `mod` lengthN xs)) xs = rotateN k xs.
+  Proof.
+    case/N.eq_0_gt_0_cases: (lengthN xs)=> H.
+    - case: xs H=> //. by rewrite !rotateN_nil.
+    - rewrite Z2N.inj_mod ?N2Z.id; try by lia.
+      by rewrite rotateN_modulo.
+  Qed.
+
+  Lemma rotateN_plus k1 k2 xs :
+    rotateN (k1 + k2) xs = rotateN k1 (rotateN k2 xs).
+  Proof. by rewrite !rotateN_iter N.iter_add. Qed.
+
+  Lemma rotateN_succ k x xs :
+    rotateN (k + 1) (x :: xs) = rotateN k (xs ++ [x]).
+  Proof. by rewrite rotateN_plus rotateN_one. Qed.
+
+  Lemma rotateN_index k xs :
+    k <= lengthN xs ->
+    rotateN k xs = dropN k xs ++ takeN k xs.
+  Proof.
+    case/N.le_lteq=> [H|->]; first by rewrite /rotateN N.mod_small//.
+    by rewrite rotateN_lengthN// dropN_lengthN// takeN_lengthN//.
+  Qed.
+
+  Lemma rotateN_mid k xs zs :
+    exists xs' zs', forall y, rotateN k (xs ++ [y] ++ zs) = xs' ++ [y] ++ zs'.
+  Proof.
+    elim/N.induction: k xs zs=> [|k IH] xs zs.
+    - exists xs. exists zs. move=> y. by rewrite rotateN_zero.
+    - rewrite -N.add_1_r. case: xs=> [|x xs].
+      + case/(_ zs []): IH=> [xs' [zs' IH]].
+        exists xs'. exists zs'. move=> y.
+        rewrite app_nil_l/= rotateN_succ.
+        by apply: IH.
+      + case/(_ xs (zs ++ [x])): IH=> [xs' [zs' IH]].
+        exists xs'. exists zs'. move=> y.
+        rewrite -app_comm_cons rotateN_succ -2!app_assoc.
+        by apply: IH.
+  Qed.
+
+  Lemma rotateN_replicateN k n x :
+    rotateN k (replicateN n x) = replicateN n x.
+  Proof. by rewrite -rotateN_fold /replicateN rotate_replicate. Qed.
+
+  Definition rotateN_simpl :=
+    (@rotateN_zero, @rotateN_one, @rotateN_succ,
+     @rotateN_modulo, @rotateN_singleton, @rotateN_replicateN).
+
+  Lemma lookupN_nil i :
+    lookupN (A := A) i [] = None.
+  Proof. rewrite /lookupN. by apply: lookup_nil. Qed.
+
+  Lemma lookupN_cons_zero x xs :
+    lookupN 0 (x :: xs) = Some x.
+  Proof. reflexivity. Qed.
+
+  Lemma lookupN_cons_succ x xs i :
+    lookupN (i + 1) (x :: xs) = lookupN i xs.
+  Proof. by rewrite /lookupN N.add_1_r N2Nat.inj_succ -lookup_tail. Qed.
+
+  Lemma lookupN_dropN xs k i :
+    lookupN i (dropN k xs) = lookupN (k + i) xs.
+  Proof. rewrite /lookupN/dropN N2Nat.inj_add. by apply: lookup_drop. Qed.
+
+  Lemma lookupN_takeN xs k i :
+    i < k ->
+    lookupN i (takeN k xs) = lookupN i xs.
+  Proof. rewrite /lookupN/takeN=> H. by apply: lookup_take; lia. Qed.
+
+  Lemma lookupN_is_Some xs i :
+    i < lengthN xs <-> is_Some (lookupN i xs).
+  Proof. rewrite /lookupN/lengthN lookup_lt_is_Some. lia. Qed.
+
+  Lemma lookupN_is_None {A'} (xs : list A') i :
+    i >= lengthN xs <-> lookupN i xs = None.
+  Proof. rewrite /lookupN/lengthN lookup_ge_None. lia. Qed.
+
+  Lemma lookupN_replicateN n x i :
+    lookupN i (replicateN n x) = Some x <-> i < n.
+  Proof.
+    rewrite /lookupN/replicateN lookup_replicate. split; [|split=> //]; lia.
+  Qed.
+
+  Lemma lookupN_head xs :
+    lookupN 0 xs = head xs.
+  Proof. by case: xs. Qed.
+
+  Lemma lookupN_tail xs i :
+    lookupN i (tail xs) = lookupN (i + 1) xs.
+  Proof. rewrite /lookupN N.add_1_r N2Nat.inj_succ. by apply: lookup_tail. Qed.
+
+  Lemma lookupN_app_l xs1 xs2 i :
+    i < lengthN xs1 ->
+    lookupN i (xs1 ++ xs2) = lookupN i xs1.
+  Proof.
+    rewrite /lookupN/lengthN=> H. by apply: lookup_app_l; lia.
+  Qed.
+
+  Lemma lookupN_app_r xs1 xs2 i :
+    i >= lengthN xs1 ->
+    lookupN i (xs1 ++ xs2) = lookupN (i - lengthN xs1) xs2.
+  Proof.
+    rewrite /lookupN/lengthN N2Nat.inj_sub Nat2N.id=> H.
+    by apply: lookup_app_r; lia.
+  Qed.
+
+  Lemma lookupN_nth_error {A'} i (xs : list A') :
+    lookupN i xs = nth_error xs (N.to_nat i).
+  Proof.
+    elim/N.induction: i xs=> [|i IH]//=; case=> [|x xs]//=.
+    - rewrite /lookupN lookup_nil. by case: (N.to_nat).
+    - rewrite N2Nat.inj_succ/= /lookupN N2Nat.inj_succ -lookup_tail/=.
+      by apply: IH.
+  Qed.
+
+  Lemma lookupN_map {B} (f : A -> B) xs i :
+    lookupN i (map f xs) = if lookupN i xs is Some x then Some (f x) else None.
+  Proof.
+    set n := lengthN xs.
+    case/decide: (i < n)=> [/lookupN_is_Some[x]/[dup]|/[dup]/lookupN_is_None].
+    - by rewrite !lookupN_nth_error=> /(map_nth_error f _ _)=> -> ->.
+    - by rewrite /n -(lengthN_map f)=> -> /lookupN_is_None ->.
+  Qed.
+
+  Lemma lookupN_rotateN xs k i :
+    i < lengthN xs ->
+    lookupN i (rotateN k xs) = lookupN ((k + i) mod lengthN xs) xs.
+  Proof.
+    rewrite /lookupN -rotateN_fold /lengthN=> H.
+    rewrite lookup_rotate_r /rotate_nat_add; last by lia.
+    f_equal. rewrite !N_nat_Z -N2Z.inj_add -nat_N_Z -N2Z.inj_mod; last by lia.
+    by rewrite -Z_N_nat N2Z.id.
+  Qed.
+
+  Lemma lookupN_any i xs :
+    A (* nonempty *) ->
+    (forall x, exists y, x <> y :> A) ->
+    (forall x, lookupN i xs = Some x) ->
+    False.
+  Proof.
+    move=> x0 H. case: (lookupN i xs)=> [y|].
+    - case/(_ y): H=> x + /(_ x) []. by apply.
+    - by case/(_ x0).
+  Qed.
+
+  Lemma lookupN_mid i xs zs :
+    A (* nonempty *) ->
+    (forall x, exists y, x <> y :> A) ->
+    (forall y, lookupN i (xs ++ [y] ++ zs) = Some y) ->
+    lengthN xs = i.
+  Proof.
+    move=> x0 H. elim/N.induction: i xs zs=> [|i IH] xs zs.
+    - case: xs=> [|x xs]//.
+      move/(_ x): H=> [y H].
+      move/(_ y). rewrite lookupN_cons_zero=> - [].
+      by [].
+    - rewrite -N.add_1_r. case: xs=> [|x xs].
+      + move=> H'. exfalso. apply: (lookupN_any i zs x0 H).
+        move=> y. move/(_ y): H'=> /=. by rewrite lookupN_cons_succ.
+      + move/(_ xs zs): IH=> IH. rewrite lengthN_cons.
+        move=> H'. f_equal. apply: IH. move=> y. rewrite -H'.
+        by rewrite -[(x :: xs) ++ _]app_comm_cons lookupN_cons_succ.
+  Qed.
+
+  Definition lookupN_simpl :=
+    (@lookupN_nil, @lookupN_cons_zero, @lookupN_cons_succ,
+     @lookupN_dropN, @lookupN_takeN,
+     @lookupN_is_Some, @lookupN_is_None,
+     @lookupN_replicateN,
+     @lookupN_tail, @lookupN_head,
+     @lookupN_app_l, @lookupN_app_r,
+     @lookupN_map,
+     @lookupN_rotateN).
 End listN.
 
 (* Not necessarily restricted to [Finite] *)
@@ -238,3 +644,11 @@ Lemma N_fin_iter_le (c : N) (P : N -> Prop) :
   Forall P (seqN 0 (N.succ c)) ->
   forall i, i <= c -> P i.
 Proof. move=> F i Hle. eapply N_fin_iter_lt; [done | lia]. Qed.
+
+Lemma N_enumerate n m :
+  n < m -> N.recursion False (fun k H => (n = k) \/ H) m.
+Proof.
+  elim/N.induction: m=> [|m']//=; first by move/N.nlt_0_r.
+  rewrite N.recursion_succ// N.lt_succ_r N.lt_eq_cases=> IH.
+  case=> [{} /IH IH|H]; by [right|left].
+Qed.
